Systems/Protocol.v
@@ -9,46 +9,11 @@ Set Implicit Arguments.
 Unset Strict Implicit.
 Unset Printing Implicit Defensive.
 
-Module Type ConsensusProtocol (P : ConsensusParams).
-Import P.
-Parameter State : Type.
-Parameter Message : Type.
-Parameter InternalTransition : Type.
+(*** TODO: Fix duplication ***)
 
-Definition peers_t := seq Address.
-Parameter Node : Address -> peers_t -> BlockTree -> TxPool -> State.
-Definition Init (n : Address) : State :=
-  Node n [:: n] (#GenesisBlock \\-> GenesisBlock) [::].
-
-(* XXX FIXME *)
-(* Need actual definitions for those. *)
-(* ... record types are a bit of a pain in modules, it seems *)
-Parameter blockTree : State -> BlockTree.
-Parameter peers : State -> peers_t.
-Parameter id : State -> Address.
-Parameter txPool : State -> TxPool.
-
-Parameter Packet : Type.
-Parameter eq_pkt : Packet -> Packet -> bool.
-Axiom eq_pktP : Equality.axiom eq_pkt.
-Canonical Packet_eqMixin := Eval hnf in EqMixin eq_pktP.
-Canonical Packet_eqType := Eval hnf in EqType Packet Packet_eqMixin.
-
-Parameter src : Packet -> Address.
-Parameter dst : Packet -> Address.
-Parameter msg : Packet -> Message.
-Definition ToSend := seq Packet.
-
-Parameter procMsg : State -> Address -> Message -> Timestamp -> State * ToSend.
-Parameter procInt : State -> InternalTransition -> Timestamp -> State * ToSend.
-
-
-End ConsensusProtocol.
-
-Module Protocol (P : ConsensusParams) (F : Forest P) <: ConsensusProtocol P.
+Module Type ConsensusProtocol (P : ConsensusParams) (F : Forest P).
 Import P F.
 
-(* Implementation of PoS protocol as a STS *)
 Definition peers_t := seq Address.
 
 Inductive _Message :=
@@ -136,11 +101,6 @@ Definition eq_msg a b :=
   | GetDataMsg _, _ => false
  end.
 
-Ltac simple_tactic mb n n' B :=
-  (case: mb=>//[|n' p'|n'|b'|t'|p' h'|p' h']; do? [by constructor 2];
-   case B: (n == n'); [by case/eqP:B=><-; constructor 1|constructor 2];
-   case=>E; subst n'; rewrite eqxx in B).
-
 (* A lot of duplication in this proof; what can be done about it? *)
 Lemma eq_msgP : Equality.axiom eq_msg.
 Proof.
@@ -170,9 +130,7 @@ Canonical Msg_eqType := Eval hnf in EqType Message Msg_eqMixin.
 End MsgEq.
 Export MsgEq.
 
-Record _Packet := mkP {src: Address; dst: Address; msg: Message}.
-Definition Packet := _Packet.
-
+Record Packet := mkP {src: Address; dst: Address; msg: Message}.
 
 Section PacketEq.
 Definition eq_pkt a b :=
@@ -200,23 +158,20 @@ Definition emitMany (packets : ToSend) := packets.
 Definition emitBroadcast (from : Address) (dst : seq Address) (msg : Message) :=
   [seq (mkP from to msg) | to <- dst].
 
-Record _State :=
-  _Node {
+Record State :=
+  Node {
     id : Address;
     peers : peers_t;
     blockTree : BlockTree;
     txPool : TxPool;
   }.
-(* This is required for module instantiation *)
-Definition Node := _Node.
-Definition State := _State.
 
 Definition Init (n : Address) : State :=
   Node n [:: n] (#GenesisBlock \\-> GenesisBlock) [::].
 Lemma peers_uniq_init (n : Address) : uniq [::n]. Proof. by []. Qed.
 
 Definition procMsg (st: State) (from : Address) (msg: Message) (ts: Timestamp) :=
-    let: _Node n prs bt pool := st in
+    let: Node n prs bt pool := st in
     match msg with
     | ConnectMsg =>
       let: ownHashes := dom bt ++ [seq hashT t | t <- pool] in
@@ -264,7 +219,461 @@ Definition procMsg (st: State) (from : Address) (msg: Message) (ts: Timestamp) :
     end.
 
 Definition procInt (st : State) (tr : InternalTransition) (ts : Timestamp) :=
-    let: _Node n prs bt pool := st in
+    let: Node n prs bt pool := st in
+    match tr with
+    | TxT tx => pair st (emitBroadcast n prs (TxMsg tx))
+
+    (* Assumption: nodes broadcast to themselves as well! => simplifies logic *)
+    | MintT =>
+      let: bc := btChain bt in
+      let: allowedTxs := [seq t <- pool | txValid t bc] in
+      match genProof n bc allowedTxs ts with
+      | Some (txs, pf) =>
+        let: prevBlock := last GenesisBlock bc in
+        let: b := mkB (hashB prevBlock) txs pf in
+        if valid_chain_block bc b then
+          let: newBt := btExtend bt b in
+          let: newPool := [seq t <- pool | txValid t (btChain newBt)] in
+          let: ownHashes := dom newBt ++ [seq hashT t | t <- newPool] in
+          pair (Node n prs newBt newPool) (emitBroadcast n prs (BlockMsg b))
+        else
+          pair st emitZero
+      | None => pair st emitZero
+      end
+    end.
+
+
+(* Proofs *)
+Lemma procMsg_id_constant (s1 : State) from (m : Message) (ts : Timestamp) :
+    id s1 = id (procMsg s1 from m ts).1.
+Proof.
+case: s1 from m ts=>n1 p1 b1 t1 from []=>//=??; last case:ifP => //=.
+- by case filter.
+- move/eqP => H_neq; case: ifP; move/eqP => //= H_eq.
+  by case ohead.
+Qed.
+
+Lemma procInt_id_constant : forall (s1 : State) (t : InternalTransition) (ts : Timestamp),
+    id s1 = id (procInt s1 t ts).1.
+Proof.
+case=> n1 p1 b1 t1 [] =>// ts; simpl.
+case hP: genProof => [[txs pf]|] //.
+case tV: (valid_chain_block _ _)=>//.
+Qed.
+
+Lemma procMsg_valid :
+   forall (s1 : State) from (m : Message) (ts : Timestamp),
+    valid (blockTree (procMsg s1 from  m ts).1) -> valid (blockTree s1).
+Proof.
+move=> s1 from  m ts.
+case Msg: m=>[||b|||]; destruct s1; rewrite/procMsg//=.
+by case filter=>//=.
+by move=>V; apply (btExtendV V).
+by case: ifP=>//= /eqP H_neq; case: ifP=>//= /eqP H_eq;
+   case filter=>//=.
+Qed.
+
+Lemma procInt_valid :
+  forall (s1 : State) (t : InternalTransition) (ts : Timestamp),
+    valid (blockTree (procInt s1 t ts).1) ->
+    valid (blockTree s1).
+Proof.
+move=>s1 t ts.
+case Int: t; destruct s1; rewrite/procInt/=; first by [].
+case: genProof => [[txs pf]|]; last done.
+case tV: (valid_chain_block _ _)=>//.
+by rewrite/blockTree/=; apply btExtendV.
+Qed.
+
+Lemma procMsg_validH :
+   forall (s1 : State) from  (m : Message) (ts : Timestamp),
+     valid (blockTree s1) -> validH (blockTree s1) ->
+     validH (blockTree (procMsg s1 from  m ts).1).
+Proof.
+move=> s1 from  m ts.
+case Msg: m=>[||b|||];
+destruct s1; rewrite/procMsg/=; do? by []; do? by case: ifP => //=.
+- by move=>v vh; case filter.
+- by move=>v vh; apply btExtendH.
+- move=>v vh; case: ifP => //=; move/eqP => H_neq; case: ifP; move/eqP => //= H_eq.
+  by case ohead.
+Qed.
+
+Lemma procInt_validH :
+   forall (s1 : State) (t : InternalTransition) (ts : Timestamp),
+     valid (blockTree s1) -> validH (blockTree s1) ->
+     validH (blockTree (procInt s1 t ts).1).
+Proof.
+move=>s1 t ts v vh.
+case Int: t; destruct s1; rewrite/procInt/=; first by [].
+case: genProof => [[txs pf]|]; last by [].
+case tV: (valid_chain_block _ _)=>//.
+by rewrite/blockTree/=; apply btExtendH.
+Qed.
+
+Lemma procMsg_has_init_block:
+   forall (s1 : State) from (m : Message) (ts : Timestamp),
+     valid (blockTree (procMsg s1 from m ts).1) -> validH (blockTree s1) ->
+     has_init_block (blockTree s1) ->
+     has_init_block (blockTree (procMsg s1 from m ts).1).
+Proof.
+move=> s1 from  m ts.
+case Msg: m=>[||b|||];
+destruct s1; rewrite/procMsg/=; do? by []; do? by case:ifP.
+- by case filter.
+- move=>V Vh Ib; apply btExtendIB=>//=.
+- move=>v vh; case: ifP => //=; move/eqP => H_neq; case: ifP; move/eqP => //= H_eq.
+  by case ohead.
+Qed.
+
+Lemma procInt_has_init_block :
+   forall (s1 : State) (t : InternalTransition) (ts : Timestamp),
+     valid (blockTree (procInt s1 t ts).1) -> validH (blockTree s1) ->
+     has_init_block (blockTree s1) ->
+     has_init_block (blockTree (procInt s1 t ts).1).
+Proof.
+move=>s1 t ts v vh ib; move: v;
+case Int: t; destruct s1; rewrite/procInt/=; first by [].
+case: genProof => [[txs pf]|]; last by [].
+case tV: (valid_chain_block _ _)=>//.
+move=>Ib; apply btExtendIB=>//=.
+Qed.
+
+Lemma procMsg_peers_uniq :
+  forall (s1 : State) from  (m : Message) (ts : Timestamp),
+    let: s2 := (procMsg s1 from m ts).1 in
+    uniq (peers s1) -> uniq (peers s2).
+Proof.
+case=> n1 p1 b1 t1 from; case; do? by []; simpl.
+- move=>? _ ?; case filter => //.
+  by move => ? ?; rewrite undup_uniq.
+- move=>_ U; case: ifP=>X; rewrite //= ?undup_uniq//=.
+  rewrite andbC/=; apply/negbT/negP; rewrite mem_undup=>Z.
+  by rewrite Z in X.
+- move=>s _ U; case: ifP => //=.
+  move/eqP => H_eq; case: ifP; move/eqP => //= H_eq'.
+  by case ohead.
+Qed.
+
+Ltac local_bc_no_change s1 hbc hbc' :=
+  (rewrite /procMsg; destruct s1=>/=; rewrite /blockTree in hbc;
+   by move=>hbc'; rewrite hbc in hbc'; rewrite hbc'; left).
+
+Lemma procMsg_non_block_nc_blockTree :
+  forall (s1 : State) from (m : Message) (ts : Timestamp),
+    let: s2 := (procMsg s1 from m ts).1 in
+    (forall b, m != BlockMsg b) ->
+    blockTree s1 = blockTree s2.
+Proof.
+move=>s1 from m ts neq.
+case: m neq=>[prs||b|t|sh|h] neq;
+  do? by[rewrite/procMsg; destruct s1=>/=].
+- by rewrite /procMsg; destruct s1 => /=; case filter.
+- by specialize (neq b); contradict neq; rewrite eqxx.
+- rewrite/procMsg/=; case: s1=>????/=; case:ifP => //=.
+  move/eqP => H_neq; case: ifP; move/eqP => //= H_eq.
+  by case ohead.
+Qed.
+
+Lemma procMsg_non_block_nc_btChain :
+  forall (s1 : State) from (m : Message) (ts : Timestamp),
+    let: s2 := (procMsg s1 from m ts).1 in
+    (forall b, m != BlockMsg b) ->
+    btChain (blockTree s1) = btChain (blockTree s2).
+Proof.
+move=>s1 from m ts neq.
+by move: (procMsg_non_block_nc_blockTree s1 from ts neq)=><-.
+Qed.
+
+Lemma procMsg_known_block_nc_blockTree :
+  forall (s1 : State) from (b : block) (ts : Timestamp),
+    let: s2 := (procMsg s1 from (BlockMsg b) ts).1 in
+    let: bt := blockTree s1 in
+    b ∈ bt -> bt = blockTree s2.
+Proof.
+move=>s1 from  b ts biT; destruct s1=>/=; rewrite/blockTree in biT.
+by apply (btExtend_withDup_noEffect biT).
+Qed.
+
+Lemma procMsg_known_block_nc_btChain (s1 : State) from (b : block) (ts : Timestamp) :
+  let: s2 := (procMsg s1 from (BlockMsg b) ts).1 in
+  let: bc := btChain (blockTree s1) in
+  valid (blockTree s1) -> has_init_block (blockTree s1) ->
+  b \in bc -> bc = btChain (blockTree s2).
+Proof.
+move=>V H biC.
+by move: (procMsg_known_block_nc_blockTree from ts (btChain_mem2 V H biC))=><-.
+Qed.
+
+Lemma procMsg_block_btExtend_bt :
+  forall (s1 : State) from (b : block) (ts: Timestamp),
+  let: s2 := (procMsg s1 from (BlockMsg b) ts).1 in
+  blockTree s2 = btExtend (blockTree s1) b.
+Proof. by move=>s1 b ts; destruct s1. Qed.
+
+Lemma procMsg_block_btExtend_btChain :
+  forall (s1 : State) from (b : block) (ts: Timestamp),
+  let: s2 := (procMsg s1 from (BlockMsg b) ts).1 in
+  btChain (blockTree s2) = btChain (btExtend (blockTree s1) b).
+Proof. by move=>s1 b ts; destruct s1. Qed.
+
+Lemma procInt_peers_uniq :
+  forall (s1 : State) (t : InternalTransition) ts, let: s2 := (procInt s1 t ts).1 in
+    uniq (peers s1) -> uniq (peers s2).
+Proof.
+move=>s1 t ts; case: s1=>n prs bt txp; rewrite /peers/procInt=>Up.
+case: t=>//; case hP: genProof => [[txs pf]|]//.
+case tV: (valid_chain_block _ _)=>//.
+Qed.
+
+Inductive local_step (s1 s2 : State) : Prop :=
+| Idle of s1 = s2
+| RcvMsg f m ts of (s2 = (procMsg s1 f m ts).1)
+| IntT t ts of (s2 = (procInt s1 t ts).1).
+
+Lemma id_constant :
+  forall (s1 s2 : State),
+    local_step s1 s2 -> id s1 = id s2.
+Proof.
+move=> s1 s2.
+case.
+- by move=> ->.
+- by move=> f m ts ->; apply procMsg_id_constant.
+- by move=> t ts ->; apply procInt_id_constant.
+Qed.
+
+Lemma bt_valid :
+  forall (s1 s2 : State),
+    local_step s1 s2 -> valid (blockTree s2) -> valid (blockTree s1).
+Proof.
+move=> s1 s2.
+case.
+- by move=> ->.
+- by move=> f m ts ->; apply procMsg_valid.
+- by move=>t ts -> V; apply (procInt_valid V).
+Qed.
+
+Lemma peers_uniq :
+  forall (s1 s2 : State),
+    uniq (peers s1) -> local_step s1 s2 -> uniq (peers s2).
+Proof.
+move=> s1 s2 UniqP1.
+case.
+- by move=> <-.
+- by move=> f m ts ->; apply procMsg_peers_uniq.
+- by move=> t ts ->; apply procInt_peers_uniq.
+Qed.
+End ConsensusProtocol.
+
+Module Protocol (P : ConsensusParams) (F : Forest P) <: ConsensusProtocol P F.
+Import P F.
+
+Definition peers_t := seq Address.
+
+Inductive _Message :=
+  | AddrMsg of peers_t
+  | ConnectMsg
+  | BlockMsg of block
+  | TxMsg of Transaction
+  | InvMsg of seq Hash
+  | GetDataMsg of Hash.
+Definition Message := _Message.
+
+Inductive _MessageType :=
+  | MAddr
+  | MConnect
+  | MBlock
+  | MTx
+  | MInv
+  | MGetData.
+Definition MessageType := _MessageType.
+
+Section MsgTypeEq.
+Definition eq_msg_type a b :=
+  match a, b with
+  | MAddr, MAddr => true
+  | MConnect, MConnect => true
+  | MBlock, MBlock => true
+  | MTx, MTx => true
+  | MInv, MInv => true
+  | MGetData, MGetData => true
+  | _, _ => false
+  end.
+
+Lemma eq_msg_typeP : Equality.axiom eq_msg_type.
+Proof.
+move=>a b; case: a; case: b; rewrite /eq_msg_type/=;
+by [constructor 1 | constructor 2].
+Qed.
+
+Canonical MsgType_eqMixin := Eval hnf in EqMixin eq_msg_typeP.
+Canonical MsgType_eqType := Eval hnf in EqType MessageType MsgType_eqMixin.
+End MsgTypeEq.
+
+Definition msg_type (msg : Message) : MessageType :=
+  match msg with
+  | AddrMsg _ => MAddr
+  | ConnectMsg => MConnect
+  | BlockMsg _ => MBlock
+  | TxMsg _ => MTx
+  | InvMsg _ => MInv
+  | GetDataMsg _ => MGetData
+  end.
+
+Definition msg_block (msg : Message) : block :=
+  match msg with
+  | BlockMsg b => b
+  | _ => GenesisBlock
+  end.
+
+Definition msg_hashes (msg : Message) : seq Hash :=
+  match msg with
+  | InvMsg sh => sh
+  | GetDataMsg h => [:: h]
+  | _ => [::]
+  end.
+
+Inductive _InternalTransition :=
+  | TxT of Transaction
+  | MintT.
+Definition InternalTransition := _InternalTransition.
+
+Module MsgEq.
+Definition eq_msg a b :=
+ match a, b with
+  | AddrMsg prsA, AddrMsg prsB => (prsA == prsB)
+  | AddrMsg _, _ => false
+  | ConnectMsg, ConnectMsg => true
+  | ConnectMsg, _ => false
+  | BlockMsg bA, BlockMsg bB => (bA == bB)
+  | BlockMsg _, _ => false
+  | TxMsg tA, TxMsg tB => (tA == tB)
+  | TxMsg _, _ => false
+  | InvMsg hA, InvMsg hB => (hA == hB)
+  | InvMsg _, _ => false
+  | GetDataMsg hA, GetDataMsg hB => (hA == hB)
+  | GetDataMsg _, _ => false
+ end.
+
+(* A lot of duplication in this proof; what can be done about it? *)
+Lemma eq_msgP : Equality.axiom eq_msg.
+Proof.
+move=> ma mb. rewrite/eq_msg.
+case: ma=>[p||b|t|h|h].
+- case: mb=>//[p'||b'|t'|h'|h']; do? [by constructor 2].
+  case B: ((p == p')).
+  - by move/eqP:B=><-; constructor 1.
+  by constructor 2; case=>Z; subst p'; rewrite eqxx in B.
+- case:mb=>////[p'||b'|t'|h'|h']; do? [by constructor 2|by constructor 1].
+- case:mb=>////[p'||b'|t'|h'|h']; do? [by constructor 2].
+  case B: (b == b'); [by case/eqP:B=><-; constructor 1|constructor 2].
+  by case=>Z; subst b'; rewrite eqxx in B.
+- case:mb=>////[p'||b'|t'|h'|h']; do? [by constructor 2].
+  case B: (t == t'); [by case/eqP:B=><-; constructor 1|constructor 2].
+  by case=>Z; subst t'; rewrite eqxx in B.
+- case:mb=>////[p'||b'|t'|h'|h']; do? [by constructor 2].
+  case B: (h == h'); [by case/eqP:B=><-; constructor 1|constructor 2].
+  by case=>Z; subst h'; rewrite eqxx in B.
+- case:mb=>////[p'||b'|t'|h'|h']; do? [by constructor 2].
+  case B: (h == h'); [by case/eqP:B=><-; constructor 1|constructor 2].
+  by case=>Z; subst h'; rewrite eqxx in B.
+Qed.
+
+Canonical Msg_eqMixin := Eval hnf in EqMixin eq_msgP.
+Canonical Msg_eqType := Eval hnf in EqType Message Msg_eqMixin.
+End MsgEq.
+Export MsgEq.
+
+Record Packet := mkP {src: Address; dst: Address; msg: Message}.
+
+Section PacketEq.
+Definition eq_pkt a b :=
+  ((src a) == (src b)) && ((dst a) == (dst b)) && ((msg a) == (msg b)).
+
+Lemma eq_pktP : Equality.axiom eq_pkt.
+Proof.
+case=>sa da ma [sb] db mb; rewrite/eq_pkt/=.
+case P1: (sa == sb)=>/=; last by constructor 2; case=>/eqP; rewrite P1.
+case P2: (da == db)=>/=; last by constructor 2; case=> _ /eqP; rewrite P2.
+case P3: (ma == mb)=>/=; last by constructor 2; case=> _ _ /eqP; rewrite P3.
+by constructor 1; move/eqP: P1=><-; move/eqP: P2=><-; move/eqP: P3=><-.
+Qed.
+
+Canonical Packet_eqMixin := Eval hnf in EqMixin eq_pktP.
+Canonical Packet_eqType := Eval hnf in EqType Packet Packet_eqMixin.
+End PacketEq.
+
+
+Definition ToSend := seq Packet.
+Definition emitZero : ToSend := [::].
+Definition emitOne (packet : Packet) : ToSend := [:: packet].
+Definition emitMany (packets : ToSend) := packets.
+
+Definition emitBroadcast (from : Address) (dst : seq Address) (msg : Message) :=
+  [seq (mkP from to msg) | to <- dst].
+
+Record State :=
+  Node {
+    id : Address;
+    peers : peers_t;
+    blockTree : BlockTree;
+    txPool : TxPool;
+  }.
+
+Definition Init (n : Address) : State :=
+  Node n [:: n] (#GenesisBlock \\-> GenesisBlock) [::].
+Lemma peers_uniq_init (n : Address) : uniq [::n]. Proof. by []. Qed.
+
+Definition procMsg (st: State) (from : Address) (msg: Message) (ts: Timestamp) :=
+    let: Node n prs bt pool := st in
+    match msg with
+    | ConnectMsg =>
+      let: ownHashes := dom bt ++ [seq hashT t | t <- pool] in
+      pair (Node n (undup (from :: prs)) bt pool)
+           (emitOne (mkP n from (InvMsg ownHashes)))
+
+    | AddrMsg knownPeers =>
+      let: newP := [seq x <- knownPeers | x \notin prs] in
+      if newP is [::] then pair st emitZero else
+      let: connects := [seq mkP n p ConnectMsg | p <- newP] in
+      let: updP := undup (prs ++ newP) in
+      pair (Node n updP bt pool) (emitMany connects ++ emitBroadcast n prs (AddrMsg updP))
+
+    | BlockMsg b =>
+      let: newBt := btExtend bt b in
+      let: newPool := [seq t <- pool | txValid t (btChain newBt)] in
+      let: ownHashes := dom newBt ++ [seq hashT t | t <- newPool] in
+      pair (Node n prs newBt newPool) (emitBroadcast n prs (InvMsg ownHashes))
+
+    | TxMsg tx =>
+      let: newPool := tpExtend pool bt tx in
+      let: ownHashes := dom bt ++ [seq hashT t | t <- newPool] in
+      pair (Node n prs bt newPool) (emitBroadcast n prs (InvMsg ownHashes))
+
+    | InvMsg peerHashes =>
+      let: ownHashes := dom bt ++ [seq hashT t | t <- pool] in
+      let: newH := [seq h <- peerHashes | h \notin ownHashes] in
+      let: gets := [seq mkP n from (GetDataMsg h) | h <- newH] in
+      pair st (emitMany gets)
+
+    | GetDataMsg h =>
+      (* Do not respond to yourself *)
+      if from == n then pair st emitZero else
+      let: matchingBlocks := [seq b <- [:: get_block bt h] | b != GenesisBlock] in
+      match ohead matchingBlocks with
+      | Some b => pair (Node n prs bt pool) (emitOne (mkP n from (BlockMsg b)))
+      | None =>
+        let: matchingTxs := [seq t <- pool | (hashT t) == h] in
+        match ohead matchingTxs with
+        | Some tx =>
+          pair (Node n prs bt pool) (emitOne (mkP n from (TxMsg tx)))
+        | None => pair st emitZero
+        end
+      end
+    end.
+
+Definition procInt (st : State) (tr : InternalTransition) (ts : Timestamp) :=
+    let: Node n prs bt pool := st in
     match tr with
     | TxT tx => pair st (emitBroadcast n prs (TxMsg tx))
 
